size.v
@@ -1,0 +1,19 @@
+Set Implicit Arguments.
+Set Asymmetric Patterns.
+
+Require Import List.
+
+Require Import comparable.
+Require Import regex.
+
+Fixpoint size {X: Set} (r: regex X) := 
+  match r with
+  | nothing => 1
+  | empty => 2
+  | char _ => 3
+  | (or s t) => 1 + size s + size t
+  | (and s t) => 1 + size s + size t
+  | (concat s t) => 1 + size s + size t
+  | (not s) => 1 + size s
+  | (zero_or_more s) => 1 + size s
+  end.
